Logic/Predicate/FirstOrder/Principia/RewriteFormula.lean
@@ -119,4 +119,111 @@ end Meta
 
 end SubFormula
 
+namespace Principia
+open SubFormula
+variable {L : Language.{u}}
+
+inductive IffFormula : (p₀ q₀ : SyntacticFormula L) → SyntacticFormula L → SyntacticFormula L → Type u
+  | intro {p₀ q₀} : IffFormula p₀ q₀ p₀ q₀
+  | reflexivity {p₀ q₀} : (p : SyntacticFormula L) → IffFormula p₀ q₀ p p
+  | and {p₀ q₀ p₁ p₂ q₁ q₂} : IffFormula p₀ q₀ p₁ q₁ → IffFormula p₀ q₀ p₂ q₂ → IffFormula p₀ q₀ (p₁ ⋏ p₂) (q₁ ⋏ q₂)
+  | or {p₀ q₀ p₁ p₂ q₁ q₂} : IffFormula p₀ q₀ p₁ q₁ → IffFormula p₀ q₀ p₂ q₂ → IffFormula p₀ q₀ (p₁ ⋎ p₂) (q₁ ⋎ q₂)
+  | all {p₀ q₀} {p q : SyntacticSubFormula L 1} : IffFormula (shift p₀) (shift q₀) (free p) (free q) → IffFormula p₀ q₀ (∀' p) (∀' q)
+  | ex {p₀ q₀} {p q : SyntacticSubFormula L 1} : IffFormula (shift p₀) (shift q₀) (free p) (free q) → IffFormula p₀ q₀ (∃' p) (∃' q)
+  | neg {p₀ q₀ p q} : IffFormula p₀ q₀ p q → IffFormula p₀ q₀ (~p) (~q)
+
+namespace IffFormula
+variable {p₀ q₀ : SyntacticFormula L}
+
+def imply (h₁ : IffFormula p₀ q₀ p₁ q₁) (h₂ : IffFormula p₀ q₀ p₂ q₂) : IffFormula p₀ q₀ (p₁ ⟶ p₂) (q₁ ⟶ q₂) :=
+  h₁.neg.or h₂
+
+def iff (h₁ : IffFormula p₀ q₀ p₁ q₁) (h₂ : IffFormula p₀ q₀ p₂ q₂) : IffFormula p₀ q₀ (p₁ ⟷ p₂) (q₁ ⟷ q₂) :=
+  (h₁.imply h₂).and (h₂.imply h₁)
+
+def toStr : IffFormula p₀ q₀ p q → String := fun _ => "rr"
+
+instance : ToString (IffFormula p₀ q₀ p q) := ⟨toStr⟩
+
+end IffFormula
+
+end Principia
+
+namespace SubFormula
+variable {L : Language.{u}}
+
+namespace Meta
+open Principia
+
+section
+variable {p₀ q₀ : SyntacticFormula L}
+
+def IffFormula_of_eq {p} (h : p₀ = p) : IffFormula p₀ q₀ p q₀ := by rw[h]; exact IffFormula.intro
+
+def IffFormula_all_of_eq (h : IffFormula p₀' q₀' p' q') (hp₀ : shift p₀ = p₀') (hq₀ : shift q₀ = q₀') (hp : free p = p') (hq : fix q' = q) :
+    IffFormula p₀ q₀ (∀' p) (∀' q) := by simp[←hp₀, ←hq₀, ←hp] at h; exact IffFormula.all (by simpa[←hq])
+
+def IffFormula_ex_of_eq (h : IffFormula p₀' q₀' p' q') (hp₀ : shift p₀ = p₀') (hq₀ : shift q₀ = q₀') (hp : free p = p') (hq : fix q' = q) :
+    IffFormula p₀ q₀ (∃' p) (∃' q) := by simp[←hp₀, ←hq₀, ←hp] at h; exact IffFormula.ex (by simpa[←hq])
+
+
+end
+
+partial def rephraseFormula {L : Q(Language.{u})} (p₀ q₀ : Q(SyntacticFormula $L)) (p : Q(SyntacticFormula $L)) :
+    MetaM ((res : Q(SyntacticFormula $L)) × Q(Principia.IffFormula $p₀ $q₀ $p $res)) := do
+  if (← isDefEq p₀ p) then
+    let eqn : Q($p₀ = $p) := (q(@rfl (SyntacticFormula $L) $p₀) : Expr)
+    return ⟨q₀, q(IffFormula_of_eq $eqn)⟩
+  else
+    match p with
+    | ~q(⊤) => return ⟨q(⊤), q(IffFormula.reflexivity _)⟩
+    | ~q(⊥) => return ⟨q(⊥), q(IffFormula.reflexivity _)⟩
+    | ~q($p ⋏ $q) => do
+      let ⟨p₁, hp⟩ ← rephraseFormula p₀ q₀ p
+      let ⟨q₁, hq⟩ ← rephraseFormula p₀ q₀ q
+      return ⟨q($p₁ ⋏ $q₁), q(IffFormula.and $hp $hq)⟩
+    | ~q($p ⋎ $q) => do
+      let ⟨p₁, hp⟩ ← rephraseFormula p₀ q₀ p
+      let ⟨q₁, hq⟩ ← rephraseFormula p₀ q₀ q
+      return ⟨q($p₁ ⋎ $q₁), q(IffFormula.or $hp $hq)⟩
+    | ~q(∀' $p) => do
+      let ⟨p₀', hp₀⟩ ← resultShift (L := L) (n := q(0)) p₀
+      let ⟨q₀', hq₀⟩ ← resultShift (L := L) (n := q(0)) q₀
+      let ⟨p', hp⟩ ← resultFree (L := L) (n := q(0)) p
+      let ⟨q', h⟩ ← rephraseFormula (L := L) p₀' q₀' p'
+      let ⟨q, hq⟩ ← resultFix (L := L) (n := q(0)) q'
+      return ⟨q(∀' $q), q(IffFormula_all_of_eq $h $hp₀ $hq₀ $hp $hq)⟩
+    | ~q(∃' $p) => do
+      let ⟨p₀', hp₀⟩ ← resultShift (L := L) (n := q(0)) p₀
+      let ⟨q₀', hq₀⟩ ← resultShift (L := L) (n := q(0)) q₀
+      let ⟨p', hp⟩ ← resultFree (L := L) (n := q(0)) p
+      let ⟨q', h⟩ ← rephraseFormula (L := L) p₀' q₀' p'
+      let ⟨q, hq⟩ ← resultFix (L := L) (n := q(0)) q'
+      return ⟨q(∃' $q), q(IffFormula_ex_of_eq $h $hp₀ $hq₀ $hp $hq)⟩
+    | ~q($p ⟶ $q) => do
+      let ⟨p₁, hp⟩ ← rephraseFormula p₀ q₀ p
+      let ⟨q₁, hq⟩ ← rephraseFormula p₀ q₀ q
+      return ⟨q($p₁ ⟶ $q₁), q(IffFormula.imply $hp $hq)⟩
+    | ~q($p ⟷ $q) => do
+      let ⟨p₁, hp⟩ ← rephraseFormula p₀ q₀ p
+      let ⟨q₁, hq⟩ ← rephraseFormula p₀ q₀ q
+      return ⟨q($p₁ ⟷ $q₁), q(IffFormula.iff $hp $hq)⟩
+    | ~q($p) => return ⟨p, q(IffFormula.reflexivity _)⟩
+
+elab "rephraseFormula" : term => do
+  let L : Q(Language.{0}) := q(Language.oring)
+  let p₀ : Q(SyntacticFormula $L) := q(“&2 < 3”)
+  let q₀ : Q(SyntacticFormula $L) := q(“&2 = 3”)
+  let p : Q(SyntacticFormula $L) := q(“&2 < 3 → ∀ (&2 + 1) + 9 * (#0 + 1)ᵀ⟦&2 + 1, 6⟧ < 0”)
+
+  let ⟨e, eq⟩ ← rephraseFormula p₀ q₀ p
+  logInfo m! "{p} \n⟹ \n{e}"
+  return eq
+
+#eval rephraseFormula
+
+end Meta
+
+end SubFormula
+
 end FirstOrder
